DEX_I/DEX_ElemLemmaNormalIntra3.v
@@ -9,6 +9,7 @@ Variable p:DEX_ExtendedProgram.
 Variable se : DEX_PC -> L.t.
 Variable reg : DEX_PC -> DEX_PC -> Prop.
 Variable m : DEX_Method.
+Variable lookupswitch_hyp : well_formed_lookupswitch m.
 
 Ltac soap2_intra_normal_aux Hreg_in H Hreg r lvl Hget_ori Hvalue_opt_in k k':=
   specialize Hreg_in with r;
@@ -35,6 +36,53 @@ Proof.
   inversion_clear Hstep' in Hpc Hst_in; subst;
   apply inv_st_in in Hst_in;
   DiscrimateEq; try (elim Hpc; reflexivity); try (contradiction).
+  (* PackedSwitch *)
+  inversion Hst_in as [Heqset Hreg_in].
+    soap2_intra_normal_aux Hreg_in H4 Hreg rt (se j) H0 Hvalue_opt_in k1 k1'.
+    (* both are low *)
+    rewrite <- H in Hvalue_opt_in; rewrite <- H5 in Hvalue_opt_in;
+      inversion Hvalue_opt_in as [v v' Hvalue_in | Hnone]; 
+      inversion Hvalue_in; subst. 
+    assert (n = n0) by omega; subst.
+    rewrite H3 in H9. inversion H9; subst; apply False_ind; auto.
+  inversion Hst_in as [Heqset Hreg_in].
+    soap2_intra_normal_aux Hreg_in H4 Hreg rt (se j) H0 Hvalue_opt_in k1 k1'.
+    (* both are low *)
+    rewrite <- H in Hvalue_opt_in; rewrite <- H6 in Hvalue_opt_in;
+      inversion Hvalue_opt_in as [v v' Hvalue_in | Hnone]; 
+      inversion Hvalue_in; subst. apply False_ind; omega.  
+  inversion Hst_in as [Heqset Hreg_in].
+    soap2_intra_normal_aux Hreg_in H3 Hreg rt (se j) H1 Hvalue_opt_in k1 k1'.
+    (* both are low *)
+    rewrite <- H0 in Hvalue_opt_in; rewrite <- H4 in Hvalue_opt_in;
+      inversion Hvalue_opt_in as [v v' Hvalue_in | Hnone]; 
+      inversion Hvalue_in; subst. apply False_ind; omega.  
+  (* SparseSwitch *)
+  inversion Hst_in as [Heqset Hreg_in].
+    soap2_intra_normal_aux Hreg_in H2 Hreg rt (se j) H0 Hvalue_opt_in k1 k1'.
+    (* both are low *)
+    rewrite <- H in Hvalue_opt_in; rewrite <- H3 in Hvalue_opt_in;
+      inversion Hvalue_opt_in as [v v' Hvalue_in | Hnone]; 
+      inversion Hvalue_in; subst.  
+      unfold well_formed_lookupswitch in lookupswitch_hyp.
+      specialize lookupswitch_hyp with (pc:=pc) (reg:=rt) (l:=l) (size:=size) (i:=Int.toZ i0) (1:=Hins) (2:=H1) (3:=H5).
+      subst. apply False_ind; auto.
+  inversion Hst_in as [Heqset Hreg_in].
+    soap2_intra_normal_aux Hreg_in H2 Hreg rt (se j) H0 Hvalue_opt_in k1 k1'.
+    (* both are low *)
+    rewrite <- H in Hvalue_opt_in; rewrite <- H4 in Hvalue_opt_in;
+      inversion Hvalue_opt_in as [v v' Hvalue_in | Hnone]; 
+      inversion Hvalue_in; subst. 
+      specialize H6 with (i':=Int.toZ i0) (o':=o) (1:=H1). 
+      apply False_ind; auto.
+  inversion Hst_in as [Heqset Hreg_in].
+    soap2_intra_normal_aux Hreg_in H3 Hreg rt (se j) H1 Hvalue_opt_in k1 k1'.
+    (* both are low *)
+    rewrite <- H0 in Hvalue_opt_in; rewrite <- H4 in Hvalue_opt_in;
+      inversion Hvalue_opt_in as [v v' Hvalue_in | Hnone]; 
+      inversion Hvalue_in; subst. 
+      specialize H2 with (i':=Int.toZ i0) (o':=o) (1:=H6). 
+      apply False_ind; omega.  
   (* If_icmp *)
   inversion Hst_in as [Heqset Hreg_in].
     (* ra *)
